PAA/PathFollowing.lean
@@ -1,0 +1,44 @@
+import PAA.PAA
+
+abbrev Cond A := A → Prop
+
+def CondAnd (P Q : Cond A) := fun s ↦ P s ∧ Q s
+
+def follow_det_cond [Ord lA] [DecidableEq lA]
+  (t : Lts_det A lA)
+  (init : A)
+  (P : List lA)
+  (C : A → Prop) :=
+  (∃ σ', Lts.follow_det t init P = some σ') ↔ C init
+
+def follow_det_cond.step [Ord lA] [DecidableEq lA]
+  (t : Lts_det A lA)
+  (init : A)
+  (P0 : lA)
+  (P : List lA)
+  (C0 C : A → Prop)
+  :
+  ((∃ σᵢ, t.step init = .some σᵢ ∧ t.label σᵢ = P0) ↔ C0 init) →
+  follow_det_cond t σᵢ P C →
+  follow_det_cond t init (P0 :: P) (CondAnd C0 C) := by
+  intro hstep hfollow
+  apply Iff.intro
+  · intro ⟨σ', hfollow'⟩
+    simp [Lts.follow_det, bind, Option.bind] at hfollow'
+    cases hstep_option : (t.step init)
+    · simp [hstep_option] at hfollow'
+    · simp [hstep_option] at hfollow'
+      rename_i σᵢ
+      simp [CondAnd]
+      apply And.intro
+      · _
+      · simp [follow_det_cond] at hfollow
+  · _
+
+def path_det_cond [Ord lA] [DecidableEq lA]
+  (t : Lts_det A lA)
+  (init : A)
+  (P : Path lA)
+  (C : A → Prop) :=
+  (∃ σ', Lts.path_det t init P = some σ') ↔ C init
+
